Let 
\begin{align}
 \vec{A}=\myvec{a\\0} ,
 \vec{B}=\myvec{b\\0},
 \vec{C}=\myvec{0\\0}
\end{align}
Since the circle passes through $\myvec{0\\0}$, the equation of given circle is,
\begin{align}
    \vec{x^\top}\vec{x}+2\vec{u^\top}\vec{x}=0 \label{quadform/july/2/1/eq:0}
\end{align}

The general equation of circle is,
\begin{align}
\vec{x^\top}\vec{x}+2\vec{u^\top}\vec{x}+f=0 
\end{align}
% Given intercepts are $\myvec{a\\0}$ and $\myvec{0\\b}$ \\
% \begin{figure}[!h]
%          \centering
%          \includegraphics[width=\columnwidth]{figure3.png}
%          \caption{Plot of the required circle}
%          \label{quadform/july/2/1/Figure}
% \end{figure}\\
Substituting $ \vec{A},  \vec{B}$ in \eqref{quadform/july/2/1/eq:0},
\begin{align}
    \vec{A^\top}\vec{A}+2\vec{u^\top}\vec{A}=0 \label{quadform/july/2/1/eq:4}
    \\
    \vec{B^\top}\vec{B}+2\vec{u^\top}\vec{B}=0 \label{quadform/july/2/1/eq:5}
\end{align}
Simplifying \eqref{quadform/july/2/1/eq:4} and \eqref{quadform/july/2/1/eq:5}
\begin{align}
    \myvec{a & 0 \\ 0 & b}\vec{u}^\top= -\frac{1}{2}\myvec{a^2 \\ b^2}
\end{align}
\begin{align}
\implies \myvec{a & 0 & -a^2/2 \\ 0 & b & -b^2/2}
\\
\xleftrightarrow [R_1\leftarrow R_1/a]{R_2\leftarrow R_2/b}
\myvec{1 & 0 & -a/2 \\ 0& 1 & -b/2}
\end{align}
\begin{align}
    \implies \vec{u}=-\frac{1}{2}\myvec{a \\ b}
     \\
     \text{or, } \vec{x^\top}\vec{x}-\myvec{a \\ b }\vec{x}=0
\end{align}
upon substituting  in \eqref{quadform/july/2/1/eq:0}.
% \begin{align}
%     \vec{x^\top}\vec{x}+2\myvec{-a/2 \\ -b/2}\vec{x}=0 
% \end{align}
% \begin{align}
 
% \end{align}
% is the desired equation of the circle.
% Substituting, $a=6$ and $b=8$,the circle is plotted.
% Equation of given circle is,
% \begin{align}
%    \implies \vec{x^\top}\vec{x}-\myvec{6 \\ 8 }\vec{x}=0
% \end{align}