%
\renewcommand{\theequation}{\theenumi}
\begin{enumerate}[label=\arabic*.,ref=\thesubsection.\theenumi]
\numberwithin{equation}{enumi}

\item	In Fig. \ref{fig:tri_med_centroid}, $BE$ and $CF$ are the medians. Show that $\triangle GEF \sim \triangle GBC$.
%
\begin{figure}[!ht]
	\begin{center}
		\resizebox{\columnwidth}{!}{\input{./figs/triangle/tri_med_centroid.tex}}
	\end{center}
	\caption{$\frac{GB}{GE} = \frac{GC}{GF} = 2$}
	\label{fig:tri_med_centroid}	
\end{figure}
\\
\solution $\because EF \parallel BC$, alternate interior angles are equal.  Hence, corresponding angles of both triangles are equal and the triangles are similar.
\item Show that

%	Using Fig. \ref{ch2_median_ratio_val}, 
	\begin{align}
\label{eq:tri_med_centroid_ratio}
	\frac{GB}{GE} = \frac{GC}{GF} = 2
	\end{align}
%
\solution $\because \triangle GEF \sim \triangle GBC$ and $\frac{EF}{BC} =2$, \eqref{eq:tri_med_centroid_ratio} follows.
%
\item In Fig. \ref{fig:tri_med_meet}, AG is extended to meet $BC$ at $D$.	Show that 
	\begin{align}
\label{eq:tri_med_centroid_ratio_AD}
\frac{GA}{GD} = 2
	\end{align}
\begin{figure}[!ht]
	\begin{center}
		\resizebox{\columnwidth}{!}{\input{./figs/triangle/tri_med_meet.tex}}
	\end{center}
	\caption{$\frac{GA}{GD} =2$}
	\label{fig:tri_med_meet}	
\end{figure}

\solution  From Theorem \ref{them:tri_med_bpt}, $ EF || BC$.  Hence,
%
\begin{align}
\triangle APE &\sim \triangle ADC \quad (AAA)
\\
\implies AP &= PD = \frac{AD}{2}
\\
\implies  AG - GP &= GP + GD 
\\
\text{or, }  GP=\frac{AG - GD}{2} 
\label{eq:tri_med_centroid_ratio_AD1}
\end{align}
%
Similarly, 
%
\begin{align}
\triangle PGE &\sim \triangle BGD  \quad (AAA)
\\
\implies \frac{GP}{GD} &= \frac{GE}{GB} = \frac{1}{2}
\\
\text{or, }  GP=\frac{GD}{2} 
\label{eq:tri_med_centroid_ratio_AD2}
\end{align}
using \eqref{eq:tri_med_centroid_ratio}. From \eqref{eq:tri_med_centroid_ratio_AD1}
and \eqref{eq:tri_med_centroid_ratio_AD2},
%
\begin{align}
GP=\frac{GA - GD}{2} &=\frac{GD}{2}  
\\
\implies  \frac{GA}{GD} &=2
\end{align}
%%
\item In Fig. 	\ref{fig:tri_med_meet_proof}, $BE$ is a median and 
%
\begin{align}
\frac{GA}{GD} &=2
\end{align}
%
Show that
%
\begin{align}
\label{eq:tri_med_final}
BD = DC
\end{align}
%%
%
\begin{figure}[!ht]
	\begin{center}
		\resizebox{\columnwidth}{!}{\input{./figs/triangle/tri_med_meet_proof.tex}}
	\end{center}
	\caption{$AD$ is also a median. }
	\label{fig:tri_med_meet_proof}	
\end{figure}
%
\\
\solution 	In Fig. \ref{fig:tri_med_meet_proof},
%
\begin{align}
\triangle GDE \sim \triangle GAB \quad (SAS)
\end{align}
%
Hence, all angles of both the above triangles are equal resulting in $DE\parallel AB$. As a consequence, 
%
\begin{align}
\triangle DDE \sim \triangle CAB \quad (AAA)
\end{align}
%
resulting in \eqref{eq:tri_med_final}

\item Medians of a triangle meet at a point.
\label{them:tri_med_meet}
\item The centroid divides the median in the ratio $2:1$.
\label{them:tri_med_ratio}
%
\item Show that 
%
\begin{align}
\vec{G} = \frac{\vec{A}+\vec{B}+\vec{C}}{3}
\end{align}
\end{enumerate}
