Given, 
\begin{align}
\vec{A}^\top=\myvec{
3 & 4 \\
-1 & 2 \\
0 & 1}\label{aug/2/17/1eq:1}\\
\Rightarrow \vec{A}=\myvec{
3 & -1 & 0 \\
4 & 2 & 1}\label{aug/2/17/1eq:2}\\
\vec{B}=\myvec{
-1 & 2 & 1\\
1 & 2 & 3}\label{aug/2/17/1eq:3}\\
\Rightarrow \vec{B}^\top=\myvec{
-1 & 1 \\
2 & 2 \\
1 & 3}\label{aug/2/17/1eq:4}
\end{align}
To verify: $\brak{\vec{A+B}}^\top=\vec{A}^\top+\vec{B}^\top$\\
From \eqref{aug/2/17/1eq:2}, \eqref{aug/2/17/1eq:3},
\begin{align}
\brak{\vec{A+B}}=\myvec{
2 & 1 & 1\\
5 & 4 & 4}\\
\therefore LHS=\brak{\vec{A+B}}^\top=\myvec{
2 & 5 \\
1 & 4 \\
1 & 4}
\end{align}
From \eqref{aug/2/17/1eq:1}, \eqref{aug/2/17/1eq:4},
\begin{align}
RHS=\vec{A}^\top+\vec{B}^\top=\myvec{
2 & 5 \\
1 & 4 \\
1 & 4}
\end{align}

