


We clearly have,
\begin{align}
\vec{A}-\vec{B} =
\myvec{
3 & 1 & 8\\
4 & 5 & 9\\
-2 & -2 & 0}
\end{align}
Therefore 
\begin{align}
(\vec{A}-\vec{B})^\top =
\myvec{
3 & 4 & -2\\
1 & 5 & -2\\
8 & 9 & 0}\label{aug/2/16/2eq:1}
\end{align}
Now,
\begin{align}
\vec{A}^\top-\vec{B}^\top &=
\myvec{
-1 & 5 & -1\\
2 & 7 & 1\\
3 & 9 & 1}-
\myvec{
-4 & 1 & 1\\
1 & 2 & 3\\
-5 & 0 & 1}\\
\vec{A}^\top-\vec{B}^\top &=
\myvec{
3 & 4 & -2\\
1 & 5 & -2\\
8 & 9 & 0}\label{aug/2/16/2eq:2}
\end{align}
Therefore from \eqref{aug/2/16/2eq:1} and \eqref{aug/2/16/2eq:2} we can conclude that $(\vec{A}-\vec{B})^\top = \vec{A}^\top-\vec{B}^\top$.




